PrimeSieve.lean
@@ -1,0 +1,11 @@
+import PrimeGen
+
+/--
+A PrimeSieve is a PrimeGen that uses a sieve to generate primes.
+In practice this means that it somehow models the set of natural
+numbers greater than 1 that are coprime to a list of primes, and
+then repeatedly:
+  - obtains the minimum of this set as the next prime
+  - eliminates multiples of the new prime. -/
+class PrimeSieve {α : Type} [PrimeGen α] where
+  todo : sorry
