RakeSieve.lean
@@ -1,3 +1,3 @@
 -- RakeSieve uses a rake to implement a prime sieve.
 import Rake
-import PrimeGen
+import PrimeSieve
