lakefile.lean
@@ -9,9 +9,10 @@ lean_lib Treesiv {
   -- add library configuration options here
 }
 
+lean_lib PrimeGen { }
+lean_lib PrimeSieve { }
 lean_lib ASeq { }
 lean_lib Rake { }
-lean_lib PrimeGen { }
 lean_lib RakeSieve { }
 
 --@[defaultTarget]
